\begin{dmath*}
R\_ss = \frac{1}{{\beta}}
\end{dmath*}
\begin{dmath*}
R\_star\_ss = (\bar{R^{*}})
\end{dmath*}
\begin{dmath*}
Y\_star\_ss = (\bar{Y^{*}})
\end{dmath*}
\begin{dmath*}
I\_ss = (\bar{I})
\end{dmath*}
\begin{dmath*}
Omega = {Lambda}_{t}\, \left(1-{\sigma}+{\sigma}\, {\psi}_{t+1}\right)
\end{dmath*}
% Equation 1
\begin{dmath}
{Lambda}_{t}=\frac{{\beta}\, \left({C}_{t}-\frac{{\zeta_{0}}\, {L}_{t}^{1+{\zeta}}}{1+{\zeta}}\right)}{{C}_{t+1}-\frac{{\zeta_{0}}\, {L}_{t+1}^{1+{\zeta}}}{1+{\zeta}}}
\end{dmath}
% Equation 2
\begin{dmath}
{\Phi}_{t}=\frac{{\kappa_{I}}}{2}\, \left(\frac{{I}_{t}}{(\bar{I})}-1\right)^{2}
\end{dmath}
% Equation 3
\begin{dmath}
{\chi^{h}}_{t}=\frac{\frac{{\varkappa_{h}}}{2}\, {K^{h}}_{t}^{2}}{{K}_{t}}
\end{dmath}
% Equation 4
\begin{dmath}
{\chi^{b}}_{t}=\frac{{\varkappa^{b}}}{2}\, {Q}_{t}\, {K^{b}}_{t}\, {x}_{t}^{2}
\end{dmath}
% Equation 5
\begin{dmath}
{\Theta(x_{t})}_{t}={\theta_{0}}\, \exp\left({x}_{t}\, \left(-{\theta}\right)\right)
\end{dmath}
% Equation 6
\begin{dmath}
{mc}_{t}=\frac{1}{{A}_{t}}\, {Z}_{t}^{{\alpha_{K}}}\, {\epsilon}_{t}^{{\alpha_{M}}}\, {w}_{t}^{1-{\alpha_{K}}-{\alpha_{M}}}
\end{dmath}
% Equation 7
\begin{dmath}
{\Pi}_{t}\, \left({\Pi}_{t}-1\right)=\frac{1}{{\kappa}}\, \left(1+{mc}_{t}\, {\eta}-{\eta}\right)+\frac{{Lambda}_{t}\, {Y}_{t+1}}{{Y}_{t}}\, {\Pi}_{t+1}\, \left({\Pi}_{t+1}-1\right)
\end{dmath}
% Equation 8
\begin{dmath}
{Y}_{t}={A}_{t}\, \left(\frac{{K}_{t-1}}{{\alpha_{K}}}\right)^{{\alpha_{K}}}\, \left(\frac{{M}_{t}}{{\alpha_{M}}}\right)^{{\alpha_{M}}}\, \left(\frac{{L}_{t}}{1-{\alpha_{K}}-{\alpha_{M}}}\right)^{1-{\alpha_{K}}-{\alpha_{M}}}
\end{dmath}
% Equation 9
\begin{dmath}
\frac{{\epsilon}_{t}\, {M}_{t}}{{Z}_{t}\, {K}_{t-1}}=\frac{{\alpha_{M}}}{{\alpha_{K}}}
\end{dmath}
% Equation 10
\begin{dmath}
\frac{{L}_{t}\, {w}_{t}}{{Z}_{t}\, {K}_{t-1}}=\frac{1-{\alpha_{K}}-{\alpha_{M}}}{{\alpha_{K}}}
\end{dmath}
% Equation 11
\begin{dmath}
{K}_{t}={I}_{t}+{K}_{t-1}\, {\lambda}
\end{dmath}
% Equation 12
\begin{dmath}
{EX}_{t}={Y^{*}}_{t}\, {\epsilon}_{t}^{{\varphi}}
\end{dmath}
% Equation 13
\begin{dmath}
\left(1-{rho\_e}\right)\, {P\_c}_{t}={kappa\_e}^{{eps\_e}_{t}+{v\_e}_{t}}
\end{dmath}
% Equation 14
\begin{dmath}
{c\_sup}_{t}={P\_c}_{t}\, {cryp}_{t}
\end{dmath}
% Equation 15
\begin{dmath}
{R\_dc}_{t}=1
\end{dmath}
% Equation 16
\begin{dmath}
{R\_c}_{t}=\frac{{P\_c}_{t}}{{P\_c}_{t-1}}
\end{dmath}
% Equation 17
\begin{dmath}
{mu\_dc}\, {DC}_{t}^{\left(-{rho\_dc}\right)}={Lambda}_{t}-\frac{{\beta}\, {Lambda}_{t+1}}{{\Pi}_{t+1}}
\end{dmath}
% Equation 18
\begin{dmath}
{mu\_m}\, {m}_{t}^{\left(-{rho\_m}\right)}={Lambda}_{t}-\frac{{\beta}\, {Lambda}_{t+1}\, {ep\_m}}{{\Pi}_{t+1}}
\end{dmath}
% Equation 19
\begin{dmath}
{mu\_c}\, {cryp}_{t}^{\left(-{rho\_cryp}\right)}={Lambda}_{t}-\frac{{R\_c}_{t}\, {\beta}\, {Lambda}_{t+1}}{{\Pi}_{t+1}}
\end{dmath}
% Equation 20
\begin{dmath}
{w}_{t}={\zeta_{0}}\, {L}_{t}^{{\zeta}}
\end{dmath}
% Equation 21
\begin{dmath}
1=\frac{{Lambda}_{t}\, \left({Z}_{t+1}+{\lambda}\, {Q}_{t+1}\right)}{{Q}_{t}+\frac{{\varkappa_{h}}\, {K^{h}}_{t}}{{K}_{t}}}
\end{dmath}
% Equation 22
\begin{dmath}
1=\frac{{Lambda}_{t}\, {R}_{t}}{{\Pi}_{t+1}}
\end{dmath}
% Equation 23
\begin{dmath}
{Q}_{t}=1+{\Phi}_{t}+\left(\frac{{I}_{t}}{(\bar{I})}-1\right)\, {\kappa_{I}}\, \frac{{I}_{t}}{(\bar{I})}
\end{dmath}
% Equation 24
\begin{dmath}
{\mu}_{t}={Lambda}_{t}\, \left(1-{\sigma}+{\sigma}\, {\psi}_{t+1}\right)\, \left(\frac{{Z}_{t+1}+{\lambda}\, {Q}_{t+1}}{{Q}_{t}}-\frac{{R}_{t}}{{\Pi}_{t+1}}\right)
\end{dmath}
% Equation 25
\begin{dmath}
{\mu^{*}}_{t}={Lambda}_{t}\, \left(1-{\sigma}+{\sigma}\, {\psi}_{t+1}\right)\, \left(\frac{{R}_{t}}{{\Pi}_{t+1}}-{R^{*}}_{t}\, \frac{{\epsilon}_{t+1}}{{\epsilon}_{t}}\right)
\end{dmath}
% Equation 26
\begin{dmath}
{\upsilon}_{t}=\frac{{Lambda}_{t}\, \left(1-{\sigma}+{\sigma}\, {\psi}_{t+1}\right)\, {R}_{t}}{{\Pi}_{t+1}}
\end{dmath}
% Equation 27
\begin{dmath}
{\phi}_{t}=\frac{{\upsilon}_{t}}{{\Theta(x_{t})}_{t}+{\upsilon}_{t}\, \frac{{\varkappa^{b}}}{2}\, {x}_{t}^{2}-\left({\mu}_{t}+{x}_{t}\, {\mu^{*}}_{t}\right)}
\end{dmath}
% Equation 28
\begin{dmath}
{\psi}_{t}={\Theta(x_{t})}_{t}\, {\phi}_{t}
\end{dmath}
% Equation 29
\begin{dmath}
{x}_{t}=\frac{{\mu^{*}}_{t}}{{\varkappa^{b}}\, {\upsilon}_{t}}-\frac{1}{{\theta}}+\sqrt{\left(\frac{{\mu^{*}}_{t}}{{\varkappa^{b}}\, {\upsilon}_{t}}\right)^{2}+\left(\frac{1}{{\theta}}\right)^{2}+\frac{2\, {\mu}_{t}}{{\varkappa^{b}}\, {\upsilon}_{t}}}
\end{dmath}
% Equation 30
\begin{dmath}
{Y}_{t}={\chi^{b}}_{t}+{\chi^{h}}_{t}+{EX}_{t}+{C}_{t}+{I}_{t}\, \left(1+{\Phi}_{t}\right)+{Y}_{t}\, \frac{{\kappa}}{2}\, \left({\Pi}_{t}-1\right)^{2}
\end{dmath}
% Equation 31
\begin{dmath}
{D^{*}}_{t}={M}_{t}+{R^{*}}_{t-1}\, {D^{*}}_{t-1}-\frac{{EX}_{t}}{{\epsilon}_{t}}
\end{dmath}
% Equation 32
\begin{dmath}
{N}_{t}={\sigma}\, \left(\left({Z}_{t}+{Q}_{t}\, {\lambda}\right)\, {K^{b}}_{t-1}-\frac{{D}_{t-1}\, {R}_{t-1}}{{\Pi}_{t}}-{D^{*}}_{t-1}\, {\epsilon}_{t}\, {R^{*}}_{t-1}\right)+{K}_{t-1}\, \left({Z}_{t}+{Q}_{t}\, {\lambda}\right)\, {\xi}
\end{dmath}
% Equation 33
\begin{dmath}
{Q}_{t}\, {K^{b}}_{t}\, \left(1+\frac{{\varkappa^{b}}}{2}\, {x}_{t}^{2}\right)={N}_{t}\, {\phi}_{t}\, \left(1+\frac{{\varkappa^{b}}}{2}\, {x}_{t}^{2}\right)
\end{dmath}
% Equation 34
\begin{dmath}
{Q}_{t}\, {K^{b}}_{t}\, \left(1+\frac{{\varkappa^{b}}}{2}\, {x}_{t}^{2}\right)={N}_{t}+{D}_{t}+{\epsilon}_{t}\, {D^{*}}_{t}
\end{dmath}
% Equation 35
\begin{dmath}
{x}_{t}=\frac{{\epsilon}_{t}\, {D^{*}}_{t}}{{Q}_{t}\, {K^{b}}_{t}}
\end{dmath}
% Equation 36
\begin{dmath}
{K}_{t}={K^{h}}_{t}+{K^{b}}_{t}
\end{dmath}
% Equation 37
\begin{dmath}
{R}_{t}-1-\left(\frac{1}{{\beta}}-1\right)={\varepsilon^{R}}_{t}+\left({\Pi}_{t}-1\right)\, \left(1-{\rho_{i}}\right)\, {\omega_{\pi}}+{\rho_{i}}\, \left({R}_{t-1}-1-\left(\frac{1}{{\beta}}-1\right)\right)
\end{dmath}
% Equation 38
\begin{dmath}
{A}_{t}=1-{\rho_{A}}+{\rho_{A}}\, {A}_{t-1}+{\varepsilon^{A}}_{t}
\end{dmath}
% Equation 39
\begin{dmath}
\log\left({eps\_e}_{t}\right)={\rho_{A}}\, \log\left({eps\_e}_{t-1}\right)
\end{dmath}
% Equation 40
\begin{dmath}
\log\left({v\_e}_{t}\right)={\rho_{A}}\, \log\left({v\_e}_{t-1}\right)
\end{dmath}
% Equation 41
\begin{dmath}
{Y^{*}}_{t}={\varepsilon^{Y*}}_{t}+{\rho_{Y*}}\, {Y^{*}}_{t-1}+(\bar{Y^{*}})\, \left(1-{\rho_{Y*}}\right)
\end{dmath}
% Equation 42
\begin{dmath}
{R^{*}}_{t}={\varepsilon^{R*}}_{t}+{R^{*}}_{t-1}\, {\rho_{R*}}+(\bar{R^{*}})\, \left(1-{\rho_{R*}}\right)
\end{dmath}
% Equation 43
\begin{dmath}
{Y^{net}}_{t}={Y}_{t}-{\epsilon}_{t}\, {M}_{t}-{Y}_{t}\, \frac{{\kappa}}{2}\, \left({\Pi}_{t}-1\right)^{2}-{\chi^{h}}_{t}-{\chi^{b}}_{t}
\end{dmath}
